feat: close to completing subst lemma

theories/Pipeline.v
@@ -1,3 +1,6 @@
+From Coq Require Import Program.
+From MetaCoq.Utils Require Import utils.
+From MetaCoq.Common Require Import Transform config.
 From MetaCoq.Erasure Require Import ExAst.
 From MetaCoq.Erasure.Typed Require Import Annotations TypeAnnotations Utils.
 From MetaCoq.ErasurePlugin Require Import Erasure Loader.
@@ -5,10 +8,9 @@ From MetaCoq.PCUIC Require Import PCUICAst.
 From MetaCoq.Template Require Import Loader TemplateMonad.
 From MetaCoq.TemplatePCUIC Require Import TemplateToPCUIC.
 From MetaCoq.SafeChecker Require Import PCUICWfEnvImpl.
-From MetaCoq.Utils Require Import utils.
-Import config.
 
-From VTL Require Import PIR Translation.
+From VTL Require PIR BigStepPIR.
+From VTL Require Import Translation.
 
 From Coq.Strings Require Import String.
 Import MCMonadNotation ListNotations.
@@ -19,9 +21,38 @@ Definition gal_id := fun x : nat => x.
 
 Definition plus_one n : nat := n + 1.
 
-(* empty_ext empty_global_env *)
+Import Common.Transform.Transform.
+
+#[local] Obligation Tactic := program_simpl.
+
+Definition pir_fuel := 5000.
+Definition pir_program := (list string * PIR.term).
+Definition eval_pir_program (p' : pir_program) (t' : PIR.term) :=
+  BigStepPIR.eval p'.2 t' 5000.
+
+Definition nom (p : EProgram.eprogram) : pir_program := ([], PIR.Var "x"%string).
+
+Program Definition box_to_pir_transform : Transform.t _ _ EAst.term PIR.term _ _
+  (EProgram.eval_eprogram EWcbvEval.default_wcbv_flags)
+  (eval_pir_program) := 
+  {| name := "translate lambda box terms into PIR terms";
+     transform p _ := nom p;
+  |}.
+Next Obligation.
+Admitted.
+Next Obligation.
+Admitted.
+Next Obligation.
+Admitted.
+Next Obligation.
+Admitted.
+Next Obligation.
+Admitted.
+
+Eval cbv in (run box_to_pir_transform).
+
+
 MetaCoq Quote Recursively Definition gid := 3.
-Eval cbv in run_erase_program typed_erasure_config  gid.
 
 Definition template_to_lt (t : Ast.term) : TemplateMonad (∑ et : EAst.term, annots box_type et) :=
   match t with
